---
layout: post
title: "Erlang & Poisson distribution"
date: 2012-03-01 10:38:06 -0500
tags: math
---
Poisson distribution (PDF):
$$
f(k;x,\lambda) = \frac{(\lambda x)^k e^{-\lambda x}}{k!}\quad\textrm{for }x,\lambda\ge 0
$$

Erlang distribution (PDF):
$$
f(x;k,\lambda) = \frac{\lambda^k x^{k-1} e^{-\lambda x}}{(k-1)!}\quad\textrm{for }x,\lambda\ge 0
$$

where $\lambda$ is the arrival rate of a Poisson process, and $k$ is the number
of arrival events. The Poisson distribution tells the probability of the number
of arrivals over a given amount of time $x$. The Erlang distribution tells the
probability of the time interval over a given number of arrivals $k$. The
difference is that, in Erlang distribution, it is assumed to have an arrival at
time $t=0$ (which is not counted toward $k$) and $t=x$ (which is counted toward
$k$), respectively, whereas Poisson does not.

## Derivation

Poisson is derived using the law of rare events: Assume $B(n,p)$ denote the
binomial distribution of $n$ Bernoulli events with "success" probability $p$.
Assume the rate of occurrence of "success" is $\lambda$, then $\lambda x = np$
where $x$ is the time to finish $n$ Bernoulli events. Define $X_n$ to be the
number of "success" events occurred. So

$$
\begin{aligned}
\lim_{n\to\infty}\Pr[X_n = k]
&= \lim_{n\to\infty}\binom{n}{k}p^k(1-p)^{n-k} \\
&= \lim_{n\to\infty}\frac{n!}{k!(n-k)!}(\frac{\lambda x}{n})^k(1-\frac{\lambda x}{n})^{n-k} \\
&= \lim_{n\to\infty}(\frac{n!}{n^k(n-k)!})\frac{(\lambda x)^k}{k!}(1-\frac{\lambda x}{n})^n(1-\frac{\lambda x}{n})^{-k} \\
&= \lim_{n\to\infty}(\frac{n(n-1)\cdots(n-(k-1))}{n^k})\frac{(\lambda x)^k}{k!}(1-\frac{\lambda x}{n})^n(1-\frac{\lambda x}{n})^{-k} \\
&= 1\cdot\frac{(\lambda x)^k}{k!}\cdot e^{-\lambda x}\cdot 1 \\
&= \frac{(\lambda x)^k}{k!}e^{-\lambda x}
\end{aligned}
$$

The formula for Erlang distribution is derived by induction. The case of
$f(x;1,\lambda)$ is trivial because this is the exponential distribution, i.e.
the time for the next arrival is $x$.

$$
\begin{aligned}
f(x;1,\lambda) &= \lambda e^{-\lambda x}  \\
&= \frac{\lambda^1 x^0 e^{-\lambda x}}{0!}
\end{aligned}
$$

Consider $f(x;k-1,\lambda)=\frac{\lambda^{k-1} x^{k-2} e^{-\lambda x}}{(k-2)!}$,
then $f(x;k,\lambda)$ is defined by the convolution:

$$
\begin{align}
f(x;k,\lambda)
&= \int_0^x f(u;k-1,\lambda)\cdot\lambda e^{-\lambda(x-u)} du \\
&= \int_0^x \frac{\lambda^{k-1} u^{k-2} e^{-\lambda u}}{(k-2)!}\cdot\lambda e^{-\lambda(x-u)} du \\
&= \frac{\lambda^k}{(k-2)!} \int_0^x u^{k-2} e^{-\lambda u} e^{-\lambda(x-u)} du \\
&= \frac{\lambda^k e^{-\lambda x}}{(k-2)!} \int_0^x u^{k-2} du \\
&= \frac{\lambda^k e^{-\lambda x}}{(k-2)!} \frac{x^{k-1}}{k-1} \\
&= \frac{\lambda^k x^{k-1} e^{-\lambda x}}{(k-1)!}
\end{align}
$$
